KeyManagement/HygienicPredicates.v
@@ -1,0 +1,50 @@
+From Coq Require Import
+     List
+     Morphisms
+     Eqdep
+     (* Program.Equality (* for dependent induction *) *)
+.
+
+Require Import
+        MyPrelude
+        Maps
+        Common
+        MapLtac
+        Keys
+        Tactics.
+
+Require Import
+        RealWorld.
+
+Set Implicit Arguments.
+
+
+
+Inductive protocol_hygienic (cs : list cipher_id): forall {A}, user_cmd A -> Prop :=
+| BindRecvHygienic :
+    forall {A t} (rec : user_cmd (message t)) (cmd : message t -> user_cmd A) pat,
+      rec = Recv pat
+      -> (forall cs' msg,
+            cs' = match msg with
+                  | SignedCiphertext _ _ c_id => c_id :: cs
+                  | _ => cs
+                  end
+            -> protocol_hygienic cs' (cmd msg))
+      -> protocol_hygienic cs (Bind rec cmd)
+| BindHygienic : forall {A B} (rec : user_cmd B) (cmd : B -> user_cmd A) b,
+    protocol_hygienic cs (cmd b)
+    -> protocol_hygienic cs (Bind rec cmd)
+| ReturnHygienic : forall {A} (a : A),
+    protocol_hygienic cs (Return a)
+| GenHygienic :
+    protocol_hygienic cs Gen
+| SendHygienic : forall {t} (uid : user_id) (msg : message t),
+    protocol_hygienic cs (Send uid msg)
+| RecvHygienic : forall {t} pat,
+    protocol_hygienic cs (@Recv t pat)
+| SignEncryptHygienic : forall {t} (msg : message t) k__s k__e,
+    protocol_hygienic cs (SignEncrypt k__s k__e msg)
+| DecryptHygienic : forall {t} msg k__s k__e c_id,
+    msg = SignedCiphertext k__s k__e c_id
+    -> List.In c_id cs
+    -> protocol_hygienic cs (@Decrypt t msg).
